Gt3/Tree/Path.lean
@@ -1,0 +1,184 @@
+import Mathlib.Data.Finset.Lattice.Fold
+
+import Gt3.Tree.Basic
+
+namespace Gt3
+
+open NumChildren BinderList HasChildren FlatChildren GetNode GetTag
+
+structure Step (α : Type _) [NumChildren α] : Type _ where
+  tag : α
+  ix : Fin (numChildren tag)
+
+def Tree.depth {α : Type _} [NumChildren α] : Tree α → ℕ
+  | .node _ children => (List.ofFn (fun i => depth (children i) + 1)).foldr max 0
+
+structure Path (α : Type _) (β : Type _ := α) : Type _ where
+  steps : List α
+  stop : β
+
+@[match_pattern]
+def Path.nil {α β : Type _} (b : β) : Path α β := { steps := [], stop := b }
+
+def Path.cons {α β : Type _} (step : α) (p : Path α β) : Path α β :=
+  { steps := step :: p.steps, stop := p.stop }
+
+def Path.length {α β : Type _} (p : Path α β) : ℕ := p.steps.length
+
+@[simp]
+theorem Path.length_nil {α β : Type _} (b : β) : (Path.nil (α := α) b).length = 0 := rfl
+
+@[simp]
+theorem Path.length_cons {α β : Type _} (step : α) (p : Path α β) :
+  (Path.cons step p).length = p.length + 1 := by simp [Path.length, Path.cons]
+
+@[simp]
+theorem Path.cons_ne_nil {α β : Type _} (step : α) (tail : Path α β) (b : β)
+  : Path.cons step tail ≠ Path.nil b :=
+  by intro h; cases h
+
+@[induction_eliminator]
+def Path.inductionOn {α β : Type _} {motive : Path α β → Sort _}
+  (nil : ∀ b, motive (.nil b))
+  (cons : ∀ (step : α) (p : Path α β), motive p → motive (Path.cons step p))
+  (p : Path α β) : motive p :=
+  match p with
+  | .mk [] stop => nil stop
+  | .mk (head::steps) stop =>
+    cons head ⟨steps, stop⟩ (inductionOn nil cons ⟨steps, stop⟩)
+
+inductive GetNode.getPaths {α τ : Type _}
+  [BinderList α] [BinderList τ] [GetTag α τ] [FlatChildren α α]
+  : α → Set (Path (Step τ) τ) where
+  | nil {t : α} : getPaths t (.nil (getTag t))
+  | cons
+      (a : α) (ix : Fin (numChildren (getTag a))) (tail : Path (Step τ) τ)
+      (htail : tail ∈ getPaths (α := α) (getChild a (ix.cast (by simp))))
+      : getPaths a (.cons (Step.mk (getTag a) ix) tail)
+
+@[simp]
+theorem GetNode.getTag_mem_getPaths {α τ : Type _}
+  [BinderList α] [BinderList τ] [GetTag α τ] [FlatChildren α α]
+  (t : α) : (.nil (getTag t)) ∈ GetNode.getPaths (α := α) t :=
+  GetNode.getPaths.nil
+
+inductive GetNode.getTraces {α τ : Type _}
+  [BinderList α] [BinderList τ] [GetTag α τ] [FlatChildren α α]
+  : α → Set (List τ) where
+  | nil {t : α} : getTraces t []
+  | cons
+      (a : α) (ix : Fin (numChildren (getTag a))) (tail : List τ)
+      (htail : tail ∈ getTraces (α := α) (getChild a (ix.cast (by simp))))
+      : getTraces a ((getTag a) :: tail)
+
+attribute [simp] getTraces.nil
+
+theorem GetNode.getPaths_node_subset {α τ : Type _} [BinderList α]
+  (t : α) [BinderList α] [BinderList τ] [GetTag α τ] [FlatChildren α α]
+  : insert (.nil (getTag t)) (⋃ i : Fin (numChildren (getTag t)),
+    { .cons (Step.mk (getTag t) i) p | p ∈ getPaths (getChild (β := α) t (i.cast (by simp))) })
+    ⊆ getPaths t
+  := by
+  intro path
+  simp only [Set.mem_insert_iff, Set.mem_iUnion, Set.mem_setOf_eq]
+  intro hpath
+  cases hpath with
+  | inl hpath => cases hpath; simp
+  | inr hpath =>
+    revert hpath
+    simp only [forall_exists_index, and_imp]
+    intro i tail htail heq
+    cases heq
+    apply GetNode.getPaths.cons
+    exact htail
+
+theorem GetNode.subset_getPaths_node {α τ : Type _} [BinderList α]
+  (t : α) [BinderList α] [BinderList τ] [GetTag α τ] [FlatChildren α α]
+  : getPaths t
+    ⊆ insert (.nil (getTag t)) (⋃ i : Fin (numChildren (getTag t)),
+      { Path.cons (Step.mk (getTag t) i) p
+        | p ∈ getPaths (getChild (β := α) t (i.cast (by simp))) })
+  := by
+  intro path hpath
+  cases hpath
+  · simp
+  case cons htail =>
+    simp only [Set.mem_insert_iff, Path.cons_ne_nil, Set.mem_iUnion, Set.mem_setOf_eq, false_or]
+    constructor
+    constructor
+    constructor
+    · exact htail
+    rfl
+
+theorem GetNode.getPaths_node {α τ : Type _} [BinderList α]
+  (t : α) [BinderList α] [BinderList τ] [GetTag α τ] [FlatChildren α α]
+  : getPaths t
+    = insert (.nil (getTag t)) (⋃ i : Fin (numChildren (getTag t)),
+      { Path.cons (Step.mk (getTag t) i) p
+        | p ∈ getPaths (getChild (β := α) t (i.cast (by simp))) })
+  := le_antisymm (subset_getPaths_node t) (getPaths_node_subset t)
+
+-- TODO: tags are obviously the same by `insert`
+
+
+-- theorem GetNode.getPaths_eq_union {α τ : Type _} [BinderList α]
+--   {t t' : α} [BinderList α] [BinderList τ] [GetTag α τ] [FlatChildren α α]
+--   (h : getPaths t = getPaths t')
+--   : (⋃ i : Fin (numChildren (getTag t)),
+--       { Path.cons (Step.mk (getTag t) i) p
+--         | p ∈ getPaths (getChild (β := α) t (i.cast (by simp))) })
+--   = (⋃ i : Fin (numChildren (getTag t')),
+--       { Path.cons (Step.mk (getTag t') i) p
+--         | p ∈ getPaths (getChild (β := α) t' (i.cast (by simp))) })
+--   := by
+--   sorry
+
+-- theorem GetNode.getPaths_eq_tag {α τ : Type _} [BinderList α]
+--   {t t' : α} [BinderList α] [BinderList τ] [GetTag α τ] [FlatChildren α α]
+--   (h : getPaths t = getPaths t')
+--   : getTag t = getTag t'
+--   := by
+--   have hu := getPaths_eq_union h
+--   simp only [Set.ext_iff, Set.mem_iUnion, Set.mem_setOf_eq] at hu
+--   sorry
+
+theorem Tree.getPaths_node_subset {α : Type _} [BinderList α]
+  (tag : α) (children : Fin (numChildren tag) → Tree α)
+  : insert (Path.nil tag)
+    (⋃ i : Fin (numChildren tag), { Path.cons (Step.mk tag i) p | p ∈ getPaths (children i) })
+    ⊆ getPaths (Tree.node tag children)
+  := GetNode.getPaths_node_subset (Tree.node tag children)
+
+-- theorem Tree.subset_getPaths_node {α : Type _} [BinderList α]
+--   (tag : α) (children : Fin (numChildren tag) → Tree α)
+--   : getPaths (Tree.node tag children)
+--     ⊆ insert [] (⋃ i : Fin (numChildren tag), { Step.mk tag i :: p | p ∈ getPaths (children i) })
+--   := GetNode.subset_getPaths_node (Tree.node tag children)
+
+theorem Tree.getPaths_node {α : Type _} [BinderList α]
+  (tag : α) (children : Fin (numChildren tag) → Tree α)
+  : getPaths (Tree.node tag children)
+    = insert (Path.nil tag)
+      (⋃ i : Fin (numChildren tag), { Path.cons (Step.mk tag i) p | p ∈ getPaths (children i) })
+  := GetNode.getPaths_node (Tree.node tag children)
+
+-- def Tree.getPaths_inj {α} [BinderList α] {t t' : Tree α} (h : getPaths t = getPaths t')
+--   : t = t' := by
+--   induction t generalizing t' with
+--   | mk tag children I =>
+--     cases t' with
+--     | mk tag' children' =>
+--       have h_union := GetNode.getPaths_eq_union h
+--       sorry
+
+def Tree.getStep {α} [NumChildren α] [DecidableEq α] (t : Tree α) (s : Step α) : Option (Tree α)
+  := if h : t.tag = s.tag then
+      some (t.children (s.ix.cast (by rw [h])))
+    else
+      none
+
+def Tree.getPath {α} [NumChildren α] [DecidableEq α] (t : Tree α) : List (Step α) → Option (Tree α)
+  | [] => some t
+  | s :: ss => (Tree.getStep t s).bind (fun t => Tree.getPath t ss)
+
+end Gt3
